% === Exercise 2.2.2 ===
\begin{Exercise}
	\begin{enumerate}[(a)]
		\item
		\begin{answer}
			$[T]_{\beta}^{\gamma} = \begin{pmatrix}
			2 & -1 \\
			3 & 4 \\
			1 & 0
			\end{pmatrix}$.
		\end{answer}
		\begin{solution}
			Since $T(1,0) = (2,3,1)$ and $T(0,1) = (-1,4,0)$.
		\end{solution}
		
		\item
		\begin{answer}
			$[T]_{\beta}^{\gamma} = \begin{pmatrix}
			2 & 3 & -1 \\
			1 & 0 & 1
			\end{pmatrix}$.
		\end{answer}
		\begin{solution}
			Since $T(1,0,0) = (2,1)$ and $T(0,1,0) = (3,0)$ and $T(0,0,1) = (-1,1)$.
		\end{solution}
		
		\item
		\begin{answer}
			$[T]_{\beta}^{\gamma} = \begin{pmatrix}
			2 & 1 & -3
			\end{pmatrix}$.
		\end{answer}
		\begin{solution}
			Since $T(1,0,0) = 2$ and $T(0,1,0) = 1$ and $T(0,0,1) = -3$.
		\end{solution}
		
		\item
		\begin{answer}
			$[T]_{\beta}^{\gamma} = \begin{pmatrix}
			0 & 2 & 1 \\
			-1 & 4 & 5 \\
			1 & 0 & 1
			\end{pmatrix}$.
		\end{answer}
		\begin{solution}
			Since $T(1,0,0) = (0,-1,1)$ and $T(0,1,0) = (2,4,0)$ and $T(0,0,1) = (1,5,1)$.
		\end{solution}
		
		\item
		\begin{answer}
			$[T]_{\beta}^{\gamma} = \begin{pmatrix}
			1 & 0 & \cdots & 0 \\
			1 & 0 & \cdots & 0 \\
			\vdots & \vdots & \ddots & \vdots \\
			1 & 0 & \cdots & 0
			\end{pmatrix}$.
		\end{answer}
		\begin{solution}
			Since $T(e_i) = e_i$ for each $i=1,2,\cdots, n$.
		\end{solution}
		
		\item
		\begin{answer}
			$[T]_{\beta}^{\gamma} = \begin{pmatrix}
			0 & \cdots & 0 & 1 \\
			0 & \cdots & 1 & 0 \\
			\vdots & \ddots & \vdots & \vdots \\
			1 & \cdots & 0 & 0
			\end{pmatrix}$.
		\end{answer}
		\begin{solution}
			Since $T(e_i) = e_{n+1-i}$ for each $i=1,2,\cdots,n$.
		\end{solution}
		
		\item
		\begin{answer}
			$[T]_{\beta}^{\gamma} = \begin{pmatrix}
			1 & 0 & \cdots & 0 & 1
			\end{pmatrix}_{1\times n}$.
		\end{answer}
		\begin{solution}
			Since
			$[T]_{\beta}^{\gamma}\begin{pmatrix}
			a_1 \\
			a_2 \\
			\vdots \\
			a_n
			\end{pmatrix}
			= a_1+a_n$.
		\end{solution}
	\end{enumerate}
\end{Exercise}