% === Exercise 2.4.2 ===
\begin{Exercise}
\begin{enumerate}[(a)]
\item[(a)]
\begin{answer}
No.
\end{answer}
\begin{solution}
Since $T$ maps $\mathbb{R}^2$ into $\mathbb{R}^3$ where $\dim(\mathbb{R}^2) = 2 \neq 3 = \dim(\mathbb{R}^3)$.
\end{solution}

\item[(b)]
\begin{answer}
No.
\end{answer}
\begin{solution}
Since $T$ maps $\mathbb{R}^2$ into $\mathbb{R}^3$ where $\dim(\mathbb{R}^2) = 2 \neq 3 = \dim(\mathbb{R}^3)$.
\end{solution}

\item[(c)]
\begin{answer}
Yes.
\end{answer}
\begin{solution}
Since
$$
T = \begin{pmatrix}
3 & 0 & -2 \\
0 & 0 & 1 \\
3 & 4 & 0
\end{pmatrix},
$$
then we have
$$
T^{-1} = \frac{1}{12}\begin{pmatrix}
4 & 8 & 0 \\
-3 & -6 & 3 \\
0 & 12 & 0
\end{pmatrix}.
$$
Hence $T^{-1}(a_1,a_2,a_3) = \frac{1}{12}(4a_1+8a_2,-3a_1-6a_2+3a_3,12a_2)$.
\end{solution}

\item[(d)]
\begin{answer}
No.
\end{answer}
\begin{solution}
Since $T$ maps $P_3(\mathbb{R})$ into $P_2(\mathbb{R})$ where $\dim(P_3(\mathbb{R})) = 4 \neq 3 = \dim(P_2(\mathbb{R}))$.
\end{solution}

\item[(e)]
\begin{answer}
No.
\end{answer}
\begin{solution}
Since $T$ maps $M_{2\times 2}(\mathbb{R})$ into $P_2(\mathbb{R})$ where $\dim(M_{2\times 2}(\mathbb{R})) = 4 \neq 3 = \dim(P_2(\mathbb{R}))$.
\end{solution}

\item[(f)]
\begin{answer}
Yes.
\end{answer}
\begin{solution}
Let $\beta := \left\{\begin{pmatrix}
1 & 0 \\
0 & 0 
\end{pmatrix}, \begin{pmatrix}
0 & 1 \\
0 & 0
\end{pmatrix}, \begin{pmatrix}
0 & 0 \\
1 & 0
\end{pmatrix}, \begin{pmatrix}
0 & 0 \\
0 & 1
\end{pmatrix} \right\}$. Put $\phi_{\beta}:M_{2\times 2}(\mathbb{R}) \to F^4$ such that $\phi_{\beta}\begin{pmatrix}
a & b \\
c & d
\end{pmatrix} = (a,b,c,d)$. And define $U:F_4\to F_4$ by $U(a,b,c,d) = (a+b,a,c,c+d)$. We know
$$
U = \begin{pmatrix}
1 & 1 & 0 & 0 \\
1 & 0 & 0 & 0 \\
0 & 0 & 1 & 0 \\
0 & 0 & 1 & 1
\end{pmatrix}.
$$
This implies
$$
U^{-1} = \begin{pmatrix}
0 & 1 & 0 & 0 \\
1 & -1 & 0 & 0 \\
0 & 0 & 1 & 0 \\
0 & 0 & -1 & 1
\end{pmatrix}.
$$
That is, $U^{-1}(a,b,c,d) = (b,a-b,c,d-c)$. Notice that $T^{-1} = \phi_{\beta}^{-1} U^{-1} \phi_{\beta}$. So
$$
T^{-1}\begin{pmatrix}
a & b \\
c & d
\end{pmatrix} = \begin{pmatrix}
b & a-b \\
c & d-c
\end{pmatrix}.
$$
\end{solution}

\end{enumerate}
\end{Exercise}