% === Exercise 3.2.6 ===
\begin{Exercise}
We pick the standard basis $\alpha$ for domain of $T$, and the standard basis $\beta$ for codomain of $T$.
\begin{enumerate}[(a)]
\item[(a)]
\begin{answer}
$[T]_{\alpha}^{\beta}$ is invertible; $[T^{-1}]_{\beta}^{\alpha} = \begin{pmatrix}
-1 & -2 & -10 \\
0 & -1 & -4 \\
0 & 0 & -1
\end{pmatrix}$.
\end{answer}
\begin{solution}
Notice that $T(a x^2 +b x+c) = -a x^2 + (4a-b)x+(2a+2b-c)$. 

Then we know $[T]_{\alpha}^{\beta}=\begin{pmatrix}
-1 & 2 & 2 \\
0 & -1 & 4 \\
0 & 0 & -1
\end{pmatrix}$.
\end{solution}

\item[(b)]
\begin{answer}
$[T]_{\alpha}^{\beta}$ is not invertible.
\end{answer}
\begin{solution}
Notice that $T(a x^2 +b x+c) = 2a x^2 + (2a+b)x+b$. 

Then we know $[T]_{\alpha}^{\beta}=\begin{pmatrix}
0 & 1 & 0 \\
0 & 1 & 2 \\
0 & 0 & 2
\end{pmatrix}$. But $\rank(T) = 2 \neq 3$.
\end{solution}

\item[(c)]
\begin{answer}
$[T]_{\alpha}^{\beta}$ is invertible; $[T^{-1}]_{\beta}^{\alpha} = \frac{1}{6}\begin{pmatrix}
1 & -2 & 3 \\
3 & 0 & -3 \\
-1 & 2 & 3
\end{pmatrix}$.
\end{answer}
\begin{solution}
We know $[T]_{\alpha}^{\beta}=\begin{pmatrix}
1 & 2 & 1 \\
-1 & 1 & 2 \\
1 & 0 & 1
\end{pmatrix}$.
\end{solution}
\end{enumerate}
\end{Exercise}