% === Exercise 6.7.6 ===
\begin{Exercise}
	Follow Exercise 6.7.3 and use Theorem 6.29 that $A^{\dagger} = V \Sigma^{\dagger} U^*$.
	\begin{enumerate}[(a)]
		\item[(a)]
		\begin{answer}
			$ A^{\dagger} = \left[\dfrac{1}{\sqrt{2}}\begin{pmatrix}
			1 & 1 \\
			1 & -1
			\end{pmatrix}\right] \begin{pmatrix}
			\sqrt{6} & 0 & 0 \\
			0 & 0 & 0
			\end{pmatrix} \left[\dfrac{1}{\sqrt{6}}\begin{pmatrix}
			\sqrt{2} & \sqrt{3} & 1 \\
			\sqrt{2} & -\sqrt{3} & 1 \\
			-\sqrt{2} & 0 & 2
			\end{pmatrix}\right]^*$.
		\end{answer}
		
		\item[(b)]
		\begin{answer}
			$ A^{\dagger} = \begin{pmatrix}
			1 & 0 & 0 \\
			0 & 0 & 1 \\
			0 & 1 & 0
			\end{pmatrix}  \begin{pmatrix}
			\sqrt{2} & 0 \\
			0 & \sqrt{2} \\
			0 & 0
			\end{pmatrix} \left[ \frac{1}{\sqrt{2}}\begin{pmatrix}
			1 & 1 \\
			1 & -1
			\end{pmatrix}\right]^*$.
		\end{answer}
	\end{enumerate}
\end{Exercise}