% === Exercise 2.5.2 ===
\begin{Exercise}
We denote the change of coordinate matrix by $Q$.
\begin{enumerate}[(a)]
\item[(a)]
\begin{answer}
$\begin{pmatrix}
a_1 & b_1 \\
a_2 & b_2
\end{pmatrix}$.
\end{answer}
\begin{solution}
Since $(a_1, a_2) = a_1 e_1 + a_2 e_2$ and $(b_1, b_2) = b_1 e_1 + b_2 e_2$. So $[(a_1,a_2)]_{\beta} = \begin{pmatrix} a_1 \\
a_2
\end{pmatrix}$ and $[(b_1,b_2)]_{\beta} = \begin{pmatrix} b_1 \\
b_2
\end{pmatrix}$. Then we know $Q = [I]_{\beta'}^{\beta} = \begin{pmatrix}
a_1 & b_1 \\
a_2 & b_2
\end{pmatrix}$.
\end{solution}

\item[(b)]
\begin{answer}
$\begin{pmatrix}
4 & 1 \\
2 & 3
\end{pmatrix}$.
\end{answer}
\begin{solution}
Since $(0,10) = 4(-1,3)+2(2,-1)$ and $(5,0) = (-1,3)+3(2,-1)$. So $[(0,10)]_{\beta} = \begin{pmatrix}
4 \\
2
\end{pmatrix}$ and $[(5,0)]_{\beta} = \begin{pmatrix} 
1 \\
3
\end{pmatrix}$. Then we know $Q = [I]_{\beta'}^{\beta} = \begin{pmatrix}
4 & 1 \\
2 & 3
\end{pmatrix}$.
\end{solution}

\item[(c)]
\begin{answer}
$\begin{pmatrix}
3 & -1 \\
5 & -2
\end{pmatrix}$.
\end{answer}
\begin{solution}
Since $(1,0) = 3(2,5)+5(-1,-3)$ and $(0,1) = -(2,5)-2(-1,-3)$. So $[e_1]_{\beta} = \begin{pmatrix}
3 \\
5
\end{pmatrix}$ and $[e_2]_{\beta} = \begin{pmatrix}
-1 \\
-2
\end{pmatrix}$. Then we know $Q = [I]_{\beta'}^{\beta} = \begin{pmatrix}
3 & -1 \\
5 & -2
\end{pmatrix}$.
\end{solution}

\item[(d)]
\begin{answer}
$\begin{pmatrix}
2 & -1 \\
5 & -4
\end{pmatrix}$.
\end{answer}
\begin{solution}
Since $(2,1) = 2(-4,3)+5(2,-1)$ and $(-4,1) = -(-4,3)-4(2,-1)$. So $[(2,1)]_{\beta} = \begin{pmatrix}
2 \\
5
\end{pmatrix}$ and $[(-4,1)]_{\beta} = \begin{pmatrix}
-1 \\
-4
\end{pmatrix}$. Then we know $Q = [I]_{\beta'}^{\beta} = \begin{pmatrix}
2 & -1 \\
5 & -4
\end{pmatrix}$.
\end{solution}

\end{enumerate}
\end{Exercise}