% === Exercise 2.5.7 ===
\begin{Exercise}
\begin{enumerate}[(a)]
\item[(a)]
\begin{answer}
$T(x,y) = \frac{1}{m^2+1}\left((1-m^2)x+2m y,2m x+(m^2-1)y\right)$.
\end{answer}
\begin{solution}
Consider the line $L:y=m x$ where $m\neq 0$. Since $(1,m)\in L$, so the reflection of $(1,m)$ over $L$ is $(1,m)$ itself. Then consider another line $L':y'=-m^{-1} x'$ such that $L\bot L'$. We observe $(-m,1)\in L'$. Notice that the reflection of $(-m,1)$ over $L$ is $(m,-1)$.

Pick $\beta' = \{(1,m),(-m,1)\}$. Also we have
$$
T(1,m) = (1,m)\text{, and } T(-m,1) = (m,-1).
$$
Since 
$$
(1,m) = (1,m)+0(m,-1) \text{, and } (m,-1) = 0(1,m)-(-m,1).
$$
It follows that $[T]_{\beta'} = \begin{pmatrix}
1 & 0 \\
0 & -1
\end{pmatrix}$. Now pick $\beta = \{e_1,e_2\}$ which is a standard basis for $\mathbb{R}^2$. So we know $[I]_{\beta'}^{\beta} = \begin{pmatrix}
1 & -m \\
m & 1
\end{pmatrix}$. Compute 
$$
[I]_{\beta}^{\beta'} = ([I]_{\beta'}^{\beta})^{-1} = \frac{1}{m^2+1}\begin{pmatrix}
1 & m \\
-m & 1
\end{pmatrix}.
$$
Hence
\begin{align*}
[T]_{\beta} 
&= [I]_{\beta'}^{\beta} [T]_{\beta'} [I]_{\beta}^{\beta'} \\
&= \begin{pmatrix}
1 & -m \\
m & 1
\end{pmatrix} \cdot \begin{pmatrix}
1 & 0 \\
0 & -1
\end{pmatrix} \cdot \frac{1}{m^2+1}\begin{pmatrix}
1 & m \\
-m & 1
\end{pmatrix} \\
&= \frac{1}{m^2+1}\begin{pmatrix}
1-m^2 & 2m \\
2m & m^2-1
\end{pmatrix}.
\end{align*}
Finally, the answer follows from $[T]_{\beta}\begin{pmatrix}
x \\
y
\end{pmatrix} = \frac{1}{m^2+1}\begin{pmatrix}
(1-m^2)x+2m y \\
2m x + (m^2-1) y
\end{pmatrix}$.
\end{solution}

\item[(b)]
\begin{answer}
$T(x,y) = \frac{1}{m^2+1}\left(x+m y,m x+m^2 y\right)$.
\end{answer}
\begin{solution}
Define $L$ and $L'$ be the same as part (a). Notice that $\mathbb{R^2} = L\oplus L'$. If $p\in \mathbb{R}^2$ such that $p=p_1+p_2$ where $p_1\in L$ and $p_2\in L'$, then $T(p) = p_1$. Since $(1,m)\in L$, then $T(1,m) = T(1,m)$; on the other hand, since $(-m,1)\in L'$, then $T(-m,1) = (0,0)$. 

Now we pick $\beta,\beta'$ which are the same as part (a). It follows that $[T]_{\beta'} = \begin{pmatrix}
1 & 0 \\
0 & 0
\end{pmatrix}$. Of course, 
$$
[I]_{\beta'}^{\beta} = \begin{pmatrix}
1 & -m \\
m & 1
\end{pmatrix}\text{, and } [I]_{\beta}^{\beta'} = \frac{1}{m^2+1}\begin{pmatrix}
1 & m \\
-m & 1
\end{pmatrix}.
$$
Hence $[T]_{\beta} = [I]_{\beta'}^{\beta} [T]_{\beta'} [I]_{\beta}^{\beta'} = \frac{1}{m^2+1}\begin{pmatrix}
1 & m \\
m & m^2
\end{pmatrix}$. 

Finally, the answer follows from $[T]_{\beta}\begin{pmatrix}
x \\
y
\end{pmatrix} = \frac{1}{m^2+1}\begin{pmatrix}
x+m y \\
m x + m^2 y
\end{pmatrix}$.
\end{solution}

\end{enumerate}
\end{Exercise}