% === Exercise 6.4.6 ===
\begin{Exercise}
	\begin{enumerate}[(a)]
		\item
		\begin{proof}
			Consider
			$$
			T_1^*
			= \left[ \frac{1}{2}(T+T^*) \right]^*
			= \frac{1}{2} (T+T^*)^*
			= \frac{1}{2} (T^*+T)
			= \frac{1}{2} (T + T^*)
			= T_1.
			$$
			This means $T_1$ is self-adjoint.
			
			Consider
			$$
			T_2^*
			= \left[ \frac{1}{2}\ii(T-T^*) \right]^*
			= \frac{1}{-2\ii}(T-T^*)^*
			= -\frac{1}{2\ii}(T^*-T)
			= \frac{1}{2\ii}(T-T^*)
			= T_2.
			$$
			This means $T_2$ is self-adjoint.
			
			Consider
			$$
			T_1 + \ii T_2
			= \frac{1}{2}(T+T^*) + \ii \cdot \frac{1}{2\ii} (T-T^*)
			= \frac{1}{2}T+ \frac{1}{2}T^* + \frac{1}{2}T - \frac{1}{2}T^*
			= T.
			$$
			We obtain the desired result.
		\end{proof}
		
		\item
		\begin{proof}
			Suppose $T = U_1+\ii U_2$ with $U_1 = U_1^*$ and $U_2 = U_2^*$.
			
			Consider
			$$
			T_1
			= \frac{1}{2}(T+T^*)
			= \frac{1}{2}(U_1 + \ii U_2 + U_1^* - \ii U_2^*)
			= \frac{1}{2}(U_1 + \ii U_2^* + U_1 - \ii U_2^*)
			= U_1.
			$$
			On the other hand,
			$$
			T_2
			= \frac{1}{2\ii}(T-T^*)
			= \frac{1}{2\ii}(U_1 + \ii U_2 - U_1^* + \ii U_2^*)
			= \frac{1}{2\ii}(U_1^*+\ii U_2 - U_1^* + \ii U_2)
			= U_2.
			$$
			
			As a result, we obtain the desired results.
		\end{proof}
		
		\item
		\begin{proof}
			$(\Longrightarrow)$
			Since $T$ is normal, then $T T^* = T^*T$. Consider
			\begin{align*}
			T_1 T_2 
			&= \frac{1}{2}(T+T^*)\cdot \frac{1}{2\ii}(T-T^*)
			= \frac{1}{4\ii}(T^2+T^* T-T T^*-T)
			= \frac{1}{4\ii}(T^2-T); \\
			T_2 T_1
			&= \frac{1}{2\ii}(T-T^*)\cdot \frac{1}{2}(T+T^*)
			= \frac{1}{4\ii}(T^2-T^*T+T T^*-T)
			= \frac{1}{4\ii}(T^2-T).
			\end{align*}
			It follows that $T_1 T_2 = T_2 T_1$.
			
			\vspace{2ex}
			
			$(\Longleftarrow)$
			Compute $T_1 T_2$ and $T_2 T_1$, since $T_1 T_2 = T_2 T_1$, we have
			$$
			\frac{1}{4\ii}(T^2+T^* T-T T^*-T)
			= \frac{1}{4\ii}(T^2-T^*T+T T^*-T).
			$$
			This implies
			$$
			2T^* T = 2T T^*.
			$$
			Then $T^* T = T T^*$ follows and hence $T$ is normal.
		\end{proof}
	\end{enumerate}
\end{Exercise}