% === Exercise 3.4.2 ===
\begin{Exercise}
	\begin{enumerate}[(a)]
		\item[(a)]
		\begin{answer}
			$(x_1,x_2,x_3) = (4,-3,-1)$.
		\end{answer}
		\begin{solution}
			$\begin{pmatrix} \left.\begin{matrix}
			1 & 2 & -1 \\
			2 & 2 & 1 \\
			3 & 5 & -2
			\end{matrix} \right| \begin{matrix}
			-1 \\
			1 \\
			-1
			\end{matrix} \end{pmatrix} \longrightarrow \begin{pmatrix} \left.\begin{matrix}
			1 & 2 & -1 \\
			0 & -2 & 3 \\
			0 & -1 & 1
			\end{matrix} \right| \begin{matrix}
			-1 \\
			3 \\
			2
			\end{matrix} \end{pmatrix} \longrightarrow \begin{pmatrix} \left.\begin{matrix}
			1 & 2 & -1 \\
			0 & -1 & 1 \\
			0 & 0 & 1
			\end{matrix} \right| \begin{matrix}
			-1 \\
			2 \\
			-1
			\end{matrix} \end{pmatrix}$. 
			
			The solution follows from
			$\left\{\begin{array}{rrrrrrrr}
			x_1 &+&2x_2&-&x_3 &=& -1 \\
			&-&x_2&+&x_3 &=& 2 \\
			& & & &x_3 &=& -1
			\end{array}\right.$. 
		\end{solution}
		
		\item[(f)]
		\begin{answer}
			$(x_1,x_2,x_3,x_4) \in \{(-3,3,1,0)+t(1,-2,0,1):t\in\mathbb{R}\}$.
		\end{answer}
		\begin{solution}
			$\begin{pmatrix} \left.\begin{matrix}
			1 & 2 & -1 & 3 \\
			2 & 4 & -1 & 6 \\
			0 & 1 & 0 & 2
			\end{matrix} \right| \begin{matrix}
			2 \\
			5 \\
			3
			\end{matrix} \end{pmatrix} \longrightarrow \begin{pmatrix} \left.\begin{matrix}
			1 & 2 & -1 & 3 \\
			0 & 1 & 0 & 2 \\
			0 & 0 & 1 & 0
			\end{matrix} \right| \begin{matrix}
			2 \\
			3 \\
			1
			\end{matrix} \end{pmatrix}$. Consider
			$$
			\left\{\begin{array}{rrrrrrrrrr}
			x_1 &+&2x_2&-&x_3 &+&3x_4 &=& 2 \\
			& &x_2&+& &+&2x_4 &=& 3 \\
			& & & &x_3 & & &=& 1
			\end{array}\right. .
			$$
			Put $x_4 = t\in\mathbb{R}$, then the solution is 
			$
			\left\{
			\begin{aligned}
			x_1 &= t-3 \\
			x_2 &= -2t+3 \\
			x_3 &= 1 \\
			x_4 &= t
			\end{aligned}\right.
			$.
			
		\end{solution}
		
	\end{enumerate}
\end{Exercise}