% === Exercise 3.4.12 ===
\begin{Exercise}
	\begin{enumerate}[(a)]
		\item
		\begin{proof}
			Since $(0,-1,0,1,1,0),(1,0,1,1,1,0)\in V$ and consider $$
			s(0,-1,0,1,1,0)+t(1,0,1,1,1,0) = (0,0,0,0,0,0).
			$$
			This leads to $s,t = 0$, we know $S$ is a linearly independent subset of $V$.
		\end{proof}
		
		\item
		\begin{solution}
			Consider
			$\begin{pmatrix}
			1 & -1 & 0 & 2 & -3 & 1 \\
			2 & -1 & -1 & 3 & -4 & 4
			\end{pmatrix} \longrightarrow \begin{pmatrix}
			1 & -1 & 0 & 2 & -3 & 1 \\
			0 & 1 & -1 & -1 & 2 & 2
			\end{pmatrix}$.
			
			We put $x_3 = a, x_4 = b,x_5 = c,x_6=d$, then
			$$
			\begin{pmatrix}
			x_1 \\
			x_2 \\
			x_3 \\
			x_4 \\
			x_5 \\
			x_6
			\end{pmatrix} = \left\{ a\begin{pmatrix}
			1 \\
			1 \\
			1 \\
			0 \\
			0 \\
			0
			\end{pmatrix} + b\begin{pmatrix}
			-1 \\
			1 \\
			0 \\
			1 \\
			0 \\
			0
			\end{pmatrix} + c\begin{pmatrix}
			1 \\
			-2 \\
			0 \\
			0 \\
			1 \\
			0
			\end{pmatrix} + d\begin{pmatrix}
			-3 \\
			-2 \\
			0 \\
			0 \\
			0 \\
			1
			\end{pmatrix} :a,b,c,d,\in\mathbb{R} \right\}.
			$$
			
			Consider the matrix
			$$
			\begin{pmatrix}
			0 & 1 & 1 & -1 & 1 & -3 \\
			-1 & 0 & 1 & 1 & -2 & -2 \\
			0 & 1 & 1 & 0 & 0 & 0 \\
			1 & 1 & 0 & 1 & 0 & 0 \\
			1 & 1 & 0 & 0 & 1 & 0 \\
			0 & 0 & 0 & 0 & 0 & 1
			\end{pmatrix}.
			$$
			Now reduce it to obtain
			$$
			\begin{pmatrix}
			0 & 1 & 1 & -1 & 1 & -3 \\
			0 & 0 & 0 & 3 & -3 & 1 \\
			0 & 0 & 0 & 1 & -1 & 3 \\
			1 & 0 & -1 & 2 & -1 & 3 \\
			0 & 0 & 0 & -1 & 1 & 0 \\
			0 & 0 & 0 & 0 & 0 & 1
			\end{pmatrix}.
			$$
			We pick the first, second, forth, sixth column to know that
			we can extend $S$ to a basis 
			$$
			\{(0,-1,0,1,1,0),(1,0,1,1,1,0),(-1,1,0,1,0,0),(-3,-2,0,0,0,1)\}
			$$
			for $V$ as desired.
		\end{solution}
		
	\end{enumerate}
\end{Exercise}