% === Exercise 2.6.3 ===
\begin{Exercise}
Let $dim(V) = n$, then we suppose $\beta^* = \{f_1,f_2,\cdots f_n\}$.
\begin{enumerate}[(a)]
\item[(a)]
\begin{answer}
$f_1(x,y,z) = x-\frac{y}{2},f_2(x,y,z) = \frac{y}{2},f_3(x,y,z) = x-z$.
\end{answer}
\begin{solution}
We should solve the systems of linear equations such that
$$
\begin{pmatrix}
1 & 0 & 1 \\
1 & 2 & 1 \\
0 & 0 & 1
\end{pmatrix} \begin{pmatrix}
f_1(e_1) & f_2(e_1) & f_3(e_1) \\
f_1(e_2) & f_2(e_2) & f_3(e_2) \\
f_1(e_3) & f_2(e_3) & f_3(e_3)
\end{pmatrix} = I_3.
$$
Hence we have
$$
\begin{pmatrix}
f_1(e_1) & f_2(e_1) & f_3(e_1) \\
f_1(e_2) & f_2(e_2) & f_3(e_2) \\
f_1(e_3) & f_2(e_3) & f_3(e_3)
\end{pmatrix} = \begin{pmatrix}
1 & 0 & -1 \\
-\frac{1}{2} & \frac{1}{2} & 0 \\
0 & 0 & 1
\end{pmatrix}.
$$
The answer follows from the change of notations.
\end{solution}

\item[(b)]
\begin{answer}
$f_1(a_0+a_1 x+a_2 x^2) = a_0,f_2(a_0+a_1 x+a_2 x^2) = a_1,f_3(a_0+a_1 x+a_2 x^2) = a_2$.
\end{answer}
\begin{solution}
We should solve the systems of linear equations such that
$$
\begin{pmatrix}
1 & 0 & 0 \\
0 & 1 & 0 \\
0 & 0 & 1
\end{pmatrix} \begin{pmatrix}
f_1(1) & f_2(1) & f_3(1) \\
f_1(x) & f_2(x) & f_3(x) \\
f_1(x^2) & f_2(x^2) & f_3(x^2)
\end{pmatrix} = I_3.
$$
Hence we have
$$
\begin{pmatrix}
f_1(1) & f_2(1) & f_3(1) \\
f_1(x) & f_2(x) & f_3(x) \\
f_1(x^2) & f_2(x^2) & f_3(x^2)
\end{pmatrix} = \begin{pmatrix}
1 & 0 & 0 \\
0 & 1 & 0 \\
0 & 0 & 1
\end{pmatrix}.
$$
The answer follows from the change of notations.
\end{solution}

\end{enumerate}
\end{Exercise}