% === Exercise 1.5.3 ===
\begin{Exercise}
	\begin{proof}
		Consider
		\begin{equation}\label{eq:1.5.3}
		a\begin{pmatrix}
		1 & 1 \\
		0 & 0 \\
		0 & 0
		\end{pmatrix} + b\begin{pmatrix}
		0 & 0 \\
		1 & 1 \\
		0 & 0
		\end{pmatrix} + c\begin{pmatrix}
		0 & 0 \\
		0 & 0 \\
		1 & 1
		\end{pmatrix} + d\begin{pmatrix}
		1 & 0 \\
		1 & 0 \\
		1 & 0
		\end{pmatrix} + e\begin{pmatrix}
		0 & 1 \\
		0 & 1 \\
		0 & 1
		\end{pmatrix} = \begin{pmatrix}
		0 & 0 \\
		0 & 0 \\
		0 & 0
		\end{pmatrix}.
		\end{equation}
		This means
		$$
		\begin{cases}
		\begin{aligned}
		a+d &= 0 \\
		a+e &= 0 \\
		b+d &= 0 \\
		b+e &= 0 \\
		c+d &= 0 \\
		c+e &= 0
		\end{aligned}
		\end{cases}.
		$$
		Hence $a=b=c$ and $d=e$ and $a+d=0$. Now we can pick $a=b=c=1$ and $d=e=-1$ so that the equation \eqref{eq:1.5.3} holds. Since $a,b,c,d,e$ are not all zeroes, by definition, we conclude the set
		$$
		\left\{\begin{pmatrix}
		1 & 1 \\
		0 & 0 \\
		0 & 0
		\end{pmatrix} , \begin{pmatrix}
		0 & 0 \\
		1 & 1 \\
		0 & 0
		\end{pmatrix} , \begin{pmatrix}
		0 & 0 \\
		0 & 0 \\
		1 & 1
		\end{pmatrix} , \begin{pmatrix}
		1 & 0 \\
		1 & 0 \\
		1 & 0
		\end{pmatrix} , \begin{pmatrix}
		0 & 1 \\
		0 & 1 \\
		0 & 1
		\end{pmatrix}\right\}
		$$
		is linearly dependent.
	\end{proof}
\end{Exercise}