% === Exercise 6.1.9 ===
\begin{Exercise}
\begin{enumerate}[(a)]
\item
\begin{proof}
Let $\beta = \{z_1,z_2,\cdots, z_n\}$, then we know $\langle x, z_i \rangle = 0$ for each $i$. Since $z\in \beta$, we have $z = \sum_{i=1}^{n} a_i z_i$ for $a_i \in F$. Consider
$$
\langle x,x \rangle
= \langle x, \sum_{i=1}^{n} a_i z_i \rangle
= \sum_{i=1}^{n} \overline{a_i} \langle x, z_i \rangle
= 0.
$$
Hence $x=0$.
\end{proof}

\item
\begin{proof}
Notice that $\langle x,z \rangle = \langle y,z \rangle$ implies $\langle x-y, z \rangle = 0$. Let $\beta = \{z_1,z_2,\cdots, z_n\}$, then we know $\langle x-y, z_i \rangle = 0$ for each $i$. From part (a), we conclude $x-y=0$ implies $x=y$.
\end{proof}
\end{enumerate}
\end{Exercise}