% === Exercise 6.1.12 ===
\begin{Exercise}
	\begin{proof}
		Since $\{v_1, v_2, \cdots, v_k\}$ is orthogonal, then $\langle v_i, v_j \rangle = 0$ for all $i\neq j$. Follow the hypothesis, then we fix $i$ to consider 
		$$
		\left\langle v_i, \sum_{j=1}^{k} a_j v_j \right\rangle
		= \sum_{j=1}^{k} \overline{a_j} \left\langle v_i, v_j \right\rangle
		= \overline{a_i}\left\langle v_i, v_i \right\rangle.
		$$
		It follows that
		\begin{align*}
		\left\| \sum_{i=1}^{k} a_i v_i \right\|^2
		&= \left\langle \sum_{i=1}^{k} a_i v_i, \sum_{j=1}^{k} a_j v_j \right\rangle \\
		&= \sum_{i=1}^{k} a_i \left\langle v_i, \sum_{j=1}^{k} a_j v_j \right\rangle \\
		&= \sum_{i=1}^{k} a_i \sum_{j=1}^{k} \overline{a_j} \left\langle v_i, v_j \right\rangle \\
		&= \sum_{i=1}^{k} a_i \overline{a_i} \left\langle v_i, v_i \right\rangle \\
		&= \sum_{i=1}^{k} |a_i|^2 \| v_i \|^2.
		\end{align*}
		We obtain the desired result.
	\end{proof}
\end{Exercise}