% === Exercise 6.1.11 ===
\begin{Exercise}
\begin{proof}
Consider for all $x,y\in V$,
\begin{align*}
\| x+y \|^2 + \| x-y \|^2
&= \sqrt{\langle x+y, x+y \rangle}^2 + \sqrt{\langle x-y, x-y \rangle}^2 \\
&= \langle x+y, x+y \rangle + \langle x-y, x-y \rangle \\
&= (\langle x,x+y \rangle + \langle y,x+y \rangle) + (\langle x,x-y \rangle - \langle y,x-y \rangle) \\
&= (\langle x,x+y \rangle + \langle x, x-y \rangle) + (\langle y,x+y \rangle + \langle y,x-y \rangle) \\
&= \langle x,2x \rangle + \langle y,2y \rangle \\
&= 2\langle x,x \rangle + 2\langle y,y \rangle \\
&= 2\|x\|^2 + 2\|y\|^2.
\end{align*}
This means that the sum of square of the four edges is
the sum of square of the two diagonals in the same parallelogram.
\end{proof}
\end{Exercise}