% === Exercise 2.3.2 ===
\begin{Exercise}
\begin{itemize}
\item Compute $A(2B+3C)$.
\begin{answer}
$$
A(2B+3C) = \begin{pmatrix}
20 & -9 & 18 \\
5 & 10 & 8
\end{pmatrix}.
$$
\end{answer}
\begin{solution}
\begin{align*}
A(2B+3C)
&= \begin{pmatrix}
1 & 3 \\
2 & -1
\end{pmatrix} \cdot \left( 2\begin{pmatrix}
1 & 0 & -3 \\
4 & 1 & 2
\end{pmatrix} + 3\begin{pmatrix}
1 & 1 & 4 \\
-1 & -2 & 0
\end{pmatrix} \right) \\
&= \begin{pmatrix}
1 & 3 \\
2 & -1
\end{pmatrix} \cdot \begin{pmatrix}
5 & 3 & 6 \\
5 & -4 & 4
\end{pmatrix} \\
&= \begin{pmatrix}
20 & -9 & 18 \\
5 & 10 & 8
\end{pmatrix}.
\end{align*}
\end{solution}

\item Compute $(A B)D$.
\begin{answer}
$$
(AB)D = \begin{pmatrix}
29 \\
-26
\end{pmatrix}.
$$
\end{answer}
\begin{solution}
\begin{align*}
(AB)D
&= \left( \begin{pmatrix}
1 & 3 \\
2 & -1
\end{pmatrix} \cdot \begin{pmatrix}
1 & 0 & -3 \\
4 & 1 & 2
\end{pmatrix} \right) \begin{pmatrix}
2 \\
-2 \\
3
\end{pmatrix} \\
&= \begin{pmatrix}
13 & 3 & 3 \\
-2 & -1 & -8
\end{pmatrix} \begin{pmatrix}
2 \\
-2 \\
3
\end{pmatrix} \\
&= \begin{pmatrix}
29 \\
-26
\end{pmatrix}.
\end{align*}
\end{solution}

\item Compute $A(B D)$.
\begin{answer}
$$
A(B D) = \begin{pmatrix}
29 \\
-26
\end{pmatrix}.
$$
\end{answer}
\begin{solution}
\begin{align*}
A(B D)
&= \begin{pmatrix}
1 & 3 \\
2 & -1
\end{pmatrix} \left( \begin{pmatrix}
1 & 0 & -3 \\
4 & 1 & 2
\end{pmatrix} \cdot \begin{pmatrix}
2 \\
-2 \\
3
\end{pmatrix} \right)\\
&= \begin{pmatrix}
1 & 3 \\
2 & -1
\end{pmatrix} \begin{pmatrix}
-7 \\
12
\end{pmatrix} \\
&= \begin{pmatrix}
29 \\
-26
\end{pmatrix}.
\end{align*}
\end{solution}

\end{itemize}
\end{Exercise}