% === Exercise 2.3.13 ===
\begin{Exercise}
	\begin{itemize}
		\item $\trace(AB) = \trace(BA)$.
	\end{itemize}
	\begin{proof}
		Consider
		\begin{gather*}
		\trace(AB)
		= \sum_{i=1}^{n} (AB)_{i i}
		= \sum_{i=1}^{n}\left( \sum_{j=1}^{n} A_{i j} B_{j i} \right)
		= \sum_{j=1}^{n} \left( \sum_{i=1}^{n} A_{i j} B_{j i} \right) \\
		= \sum_{j=1}^{n} \left( \sum_{i=1}^{n} B_{j i} A_{i j}  \right)
		= \sum_{j=1}^{n} (BA)_{j j}
		= \trace(BA).
		\end{gather*}
		Hence we obtain what to prove.
	\end{proof}
	
	\begin{itemize}
		\item $\trace(A) = \trace(A^t)$.
	\end{itemize}
	\begin{proof}
		Notice that $A_{i j} = A^t_{j i}$ for all $i,j$. So $A_{i i} = A^t_{i i}$.
		Consider
		$$
		\trace(A)
		= \sum_{i=1}^{n} A_{i i}
		= \sum_{i=1}^{n} A^t_{i i}
		= \trace(A^t).
		$$
		Hence we obtain what to prove.
	\end{proof}
\end{Exercise}