% === Exercise 1.1.1 ===
\begin{Exercise}
\begin{enumerate}[(a)]
\item 
\begin{answer}
No.
\end{answer}
\begin{solution}
Since there is no real number $k\neq 0$ such that $(3,1,2)=k(6,4,2)$.
\end{solution}

\item
\begin{answer}
Yes.
\end{answer}
\begin{solution}
Since $(9,-3,-21) = -3(-3,1,7)$.
\end{solution}

\item
\begin{answer}
Yes.
\end{answer}
\begin{solution}
Since $(5,-6,7) = -1(-5,6,-7)$.
\end{solution}

\item
\begin{answer}
No.
\end{answer}
\begin{solution}
Since there is no real number $k\neq 0$ such that $(2,0,-5)=k(5,0,-2)$.
\end{solution}
\end{enumerate}
\end{Exercise}