% === Exercise 1.1.2 ===
\begin{Exercise}
	\begin{enumerate}[(a)]
		\item
		\begin{answer}
			$(3,-2,4) + t(-8,9,-3)$ for $t\in\mathbb{R}$.
		\end{answer}
		\begin{solution}
			Notice that $(-8,9,-3) = (-5,7,1) - (3,-2,4)$.
		\end{solution}
		
		\item 
		\begin{answer}
			$(2,4,0) + t(-5,-10,0)$ for $t\in\mathbb{R}$.
		\end{answer}
		\begin{solution}
			Notice that $(-5,-10,0) = (-3,-6,0) - (2,4,0)$.
		\end{solution}
		
		\item 
		\begin{answer}
			$(3,7,2) + t(0,0,-10)$ for $t\in\mathbb{R}$.
		\end{answer}
		\begin{solution}
			Notice that $(0,0,-10) = (3,7,-8) - (3,7,2)$.
		\end{solution}
		
		\item
		\begin{answer}
			$(-2,-1,5) + t(5,10,2)$ for $t\in\mathbb{R}$.
		\end{answer}
		\begin{solution}
			Notice that $(5,10,-2) = (3,9,7) - (-2,-1,5)$.
		\end{solution}
	\end{enumerate}
\end{Exercise}