% === Exercise 1.1.3 ===
\begin{Exercise}
\begin{enumerate}[(a)]
\item 
\begin{answer}
$(2,-5,-1)+s(-2,9,7)+t(-5,12,2)$ for $s,t\in\mathbb{R}$.
\end{answer}
\begin{solution}
Let $A := (2,-5,-1), B := (0,4,6), C := (-3,7,1)$.

Since $\overrightarrow{AB} = (-2,9,7)$ and $\overrightarrow{AC} = (-5,12,2)$, then the equation of the plane is $A+s\overrightarrow{AB}+t\overrightarrow{AC} = (2,-5,-1)+s(-2,9,7)+t(-5,12,2)$ for $s,t\in\mathbb{R}$.
\end{solution}

\item 
\begin{answer}
$(3,-6,7)+s(-5,6,-11)+t(2,-3,-9)$ for $s,t\in\mathbb{R}$.
\end{answer}
\begin{solution}
Let $A := (3,-6,7), B := (-2,0,-4), C := (5,-9,-2)$.

Since $\overrightarrow{AB} = (-5,6,-11)$ and $\overrightarrow{AC} = (2,-3,-9)$, then the equation of the plane is $A+s\overrightarrow{AB}+t\overrightarrow{AC} = (3,-6,7)+s(-5,6,-11)+t(2,-3,-9)$ for $s,t\in\mathbb{R}$.
\end{solution}

\item 
\begin{answer}
$(-8,2,0)+s(9,1,0)+t(14,-7,0)$ for $s,t\in\mathbb{R}$.
\end{answer}
\begin{solution}
Let $A := (-8,2,0), B := (1,3,0), C := (6,-5,0)$.

Since $\overrightarrow{AB} = (9,1,0)$ and $\overrightarrow{AC} = (14,-7,0)$, then the equation of the plane is $A+s\overrightarrow{AB}+t\overrightarrow{AC} = (-8,2,0)+s(9,1,0)+t(14,-7,0)$ for $s,t\in\mathbb{R}$.
\end{solution}

\item 
\begin{answer}
$(1,1,1)+s(4,4,4)+t(-7,3,1)$ for $s,t\in\mathbb{R}$.
\end{answer}
\begin{solution}
Let $A := (1,1,1), B := (5,5,5), C := (-6,4,2)$.

Since $\overrightarrow{AB} = (4,4,4)$ and $\overrightarrow{AC} = (-7,3,1)$, then the equation of the plane is $A+s\overrightarrow{AB}+t\overrightarrow{AC} = (1,1,1)+s(4,4,4)+t(-7,3,1)$ for $s,t\in\mathbb{R}$.
\end{solution}
\end{enumerate}
\end{Exercise}