% === Exercise 1.4.5 ===
\begin{Exercise}
\begin{enumerate}[(a)]
\item[(a)]
\begin{answer}
Yes.
\end{answer}
\begin{solution}
Consider
$$
a(1,0,2)+b(-1,1,1) = (2,-1,1).
$$
This implies
$$
\begin{cases}
\begin{aligned}
a-b &= 2 \\
b &= -1 \\
2a+b &= 1
\end{aligned}
\end{cases}.
$$
Solve to obtain
$$
\begin{cases}
\begin{aligned}
a &= 1 \\
b &= -1
\end{aligned}
\end{cases}.
$$
Hence $(2,-1,1) = (1,0,2)-(-1,1,1) \in span(S)$.
\end{solution}

\item[(b)]
\begin{answer}
No.
\end{answer}
\begin{solution}
Consider
$$
a(1,0,2)+b(-1,1,1) = (-1,2,1).
$$
This implies
$$
\begin{cases}
\begin{aligned}
a-b &= -1 \\
b &= 2 \\
2a+b &= 1
\end{aligned}
\end{cases}.
$$
This systems of linear equations has no solution. Hence $(-1,2,1)\notin span(S)$.
\end{solution}

\item[(c)]
\begin{answer}
No.
\end{answer}
\begin{solution}
Consider
$$
a(1,0,1,-1)+b(0,1,1,1) = (-1,1,1,2).
$$
This implies
$$
\begin{cases}
\begin{aligned}
a &= -1 \\
b &= 1 \\
a+b &= 1 \\
-a+b &= 2
\end{aligned}
\end{cases}.
$$
This systems of linear equations has no solution. Hence $(-1,1,1,2)\notin span(S)$.
\end{solution}

\item[(d)]
\begin{answer}
Yes.
\end{answer}
\begin{solution}
Consider
$$
a(1,0,1,-1)+b(0,1,1,1) = (2,-1,1,-3).
$$
This implies
$$
\begin{cases}
\begin{aligned}
a &= 2 \\
b &= -1 \\
a+b &= 1 \\
-a+b &= -3
\end{aligned}
\end{cases}.
$$
Hence $(2,-1,1,-3) = 2(1,0,1,-1)-(0,1,1,1) \in span(S)$.
\end{solution}

\item[(e)]
\begin{answer}
Yes.
\end{answer}
\begin{solution}
Consider
$$
a(x^3+x^2+x+1)+b(x^2+x+1)+c(x+1) = -x^3+2x^2+3x+3.
$$
This implies
$$
\begin{cases}
\begin{aligned}
a &= -1 \\
a+b &= 2 \\
a+b+c &= 3 \\
a+b+c &= 3
\end{aligned}
\end{cases}.
$$
Solve to obtain $a=-1,b=3,c=1$. Hence 
$$
-x^3+2x^2+3x+3=-(x^3+x^2+x+1)+3(x^2+x+1)+(x+1)\in span(S).
$$
\end{solution}

\item[(f)]
\begin{answer}
No.
\end{answer}
\begin{solution}
Consider
$$
a(x^3+x^2+x+1)+b(x^2+x+1)+c(x+1) = 2x^3-x^2+x+3.
$$
This implies
$$
\begin{cases}
\begin{aligned}
a &= 2 \\
a+b &= -1 \\
a+b+c &= 1 \\
a+b+c &= 3
\end{aligned}
\end{cases}.
$$
This system of linear equations have no solution. Hence $2x^3-x^2+x+3\notin span(S)$.
\end{solution}

\item[(g)]
\begin{answer}
Yes.
\end{answer}
\begin{solution}
Consider
$$
a\begin{pmatrix}
1 & 0 \\
-1 & 0
\end{pmatrix} + b\begin{pmatrix}
0 & 1 \\
0 & 1
\end{pmatrix} + c\begin{pmatrix}
1 & 1 \\
0 & 0
\end{pmatrix} = \begin{pmatrix}
1 & 2 \\
-3 & 4
\end{pmatrix}.
$$
This implies
$$
\begin{cases}
\begin{aligned}
a+c &= 1 \\
b+c &= 2 \\
-a &= -3 \\
b &= 4
\end{aligned}
\end{cases}.
$$
Solve to obtain $a=3,b=4,c=-2$. Hence
$$
\begin{pmatrix}
1 & 2 \\
-3 & 4
\end{pmatrix} \in span(S).
$$
\end{solution}

\item[(h)]
\begin{answer}
No.
\end{answer}
\begin{solution}
Consider
$$
a\begin{pmatrix}
1 & 0 \\
-1 & 0
\end{pmatrix} + b\begin{pmatrix}
0 & 1 \\
0 & 1
\end{pmatrix} + c\begin{pmatrix}
1 & 1 \\
0 & 0
\end{pmatrix} = \begin{pmatrix}
1 & 0 \\
0 & 1
\end{pmatrix}.
$$
This implies
$$
\begin{cases}
\begin{aligned}
a+c &= 1 \\
b+c &= 0 \\
-a &= 0 \\
b &= 1
\end{aligned}
\end{cases}.
$$
This system of linear equations have no solution. Hence 
$$
\begin{pmatrix}
1 & 0 \\
0 & 1
\end{pmatrix} \notin span(S).
$$
\end{solution}
\end{enumerate}
\end{Exercise}