
% === Exercise 2.1.35 ===
\begin{Exercise}
	\begin{enumerate}[(a)]
		\item
		\begin{proof}
			Notice that $V$ is finite-dimensional vector space. then both $\nullity(T)$ and $\rank(T)$ are finite. By hypothesis $V=R(T)+N(T)$, it suffices to prove $R(T)\cap N(T) = \{0\}$.
			
			By Exercise 1.6.29(a), we know 
			$$
			\dim(R(T)+N(T)) = \dim(R(T))+\dim(N(T))-\dim(R(T)\cap N(T)).
			$$
			By hypothesis, we have
			$$
			\dim(R(T)\cap N(T)) = \dim(R(T))+\dim(N(T))-\dim(V).
			$$
			Since $\dim(V)$ is finite, by the Dimension Theorem, we have
			$$
			\dim(V) = \rank(T)+ \nullity(T) = \dim(R(T))+\dim(N(T)).
			$$
			Finally we obtain
			$$
			\dim(R(T)\cap N(T)) = 0
			$$
			which implies
			$$
			R(T)\cap N(T) = \{0\}.
			$$
			Hence
			$$
			V = R(T)\oplus N(T).
			$$
		\end{proof}
		
		\item
		\begin{proof}
			This is similar to part (a). Notice that $\dim(V)$ is finite, then both $\nullity(T)$ and $\rank(T)$ are finite. Consider
			$$
			\dim(R(T)+N(T)) = \dim(R(T))+\dim(N(T))-\dim(R(T)\cap N(T)).
			$$
			By hypothesis, we know
			$$
			\dim(R(T)+N(T)) = \dim(R(T))+\dim(N(T))-0.
			$$
			By the Dimension Theorem, we have
			$$
			\dim(R(T)+N(T)) = \dim(R(T))+\dim(N(T)) = \dim(V).
			$$
			Hence $R(T)+N(T) = V$. Then following $R(T)\cap N(T) = \{0\}$ by hypothesis, we conclude
			$$
			V = R(T)\oplus N(T).
			$$
		\end{proof}
	\end{enumerate}
\end{Exercise}