% === Exercise 2.1.22 ===
\begin{Exercise}
	\begin{itemize}
		\item $T:\mathbb{R}^3\to\mathbb{R}$ is linear
	\end{itemize}
	\begin{proof}
		Let $\beta := \{e_1, e_2, e_3\}$ be a basis for $\mathbb{R}^3$.
		Set $T(e_1) = a$, $T(e_2) = b$, $T(e_3) = c$.
		For any $(x,y,z)\in\mathbb{R}^3$, we have
		$$
		T(x,y,z) 
		= T(x e_1+y e_2+z e_3) 
		= x T(e_1)+y T(e_2)+ z T(e_3)
		= a x+b y+c z.
		$$
	\end{proof}
	
	\begin{itemize}
		\item $T:F^n\to F$ is linear
	\end{itemize}
	\begin{proof}
		Let $\beta := \{e_1, \cdots, e_n\}$ be a basis for $F^n$.
		Set $T(e_i) = c_i\in F$ for each $i=1,\cdots,n$.
		For any $(x_1,\cdots,x_n)\in F^n$, we have
		$$
		T(x_1, \cdots, x_n)
		= T(x_1 e_1+\cdots, x_n e_n)
		= x_1 T(e_1)+\cdots+x_n T(e_n)
		= c_1 x_1 + \cdots c_n x_n.
		$$
	\end{proof}
	
	\begin{itemize}
		\item $T:F^n\to F^m$ is linear
	\end{itemize}
	\begin{proof}
		Let $\beta := \{e_1, \cdots, e_n\}$ be a basis for $F^n$.
		Set $T(e_i) = \sum_{j=1}^{m} c_{i j} w_j\in F$ for each $i=1,\cdots,n$.
		For any $(x_1,\cdots,x_n)\in F^n$, we have
		\begin{align*}
		T(x_1,\cdots, x_n)
		&= T\left( \sum_{i=1}^{n} x_i e_i \right) \\
		&= \sum_{i=1}^{n} x_i T(e_i) \\
		&= \sum_{i=1}^{n} x_i \sum_{j=1}^{m} c_{i j} w_j \\
		&= \sum_{i=1}^{n} \sum_{j=1}^{m} c_{i j} x_i w_j \\
		&= \sum_{j=1}^{m} \left( \sum_{i=1}^{n} c_{i j} x_i \right) w_j \\
		&= (\sum_{i=1}^{n} c_{i 1} x_1, \cdots, \sum_{i=1}^{n} c_{i m} x_m).
		\end{align*}
	\end{proof}
\end{Exercise}