% === Exercise 1.3.29 ===
\begin{Exercise}
	\begin{proof}
		Let $A\in M_{n\times n}(F)$ arbitrarily. And then pick $B\in W_2$ arbitrarily. We know $A-B\in W_1$. Consider
		\begin{align*}
			A 
			&= (A-B) + B \\
			&\in \left\{ x+y:x\in W_1\text{ and }y\in W_2 \right\} \\
			&= W_1+W_2.
		\end{align*}
		By the arbitrary choice of $A$, we know $M_{n\times n}(F)\subseteq W_1+W_2$.
		
		On the other hand, $W_1+W_2\subseteq M_{n\times n}(F)$ trivially. Hence 
		$$
		W_1+W_2 = M_{n\times n}(F).
		$$
		
		Notice that
		\begin{align*}
			W_1\cap W_2
			&= \left\{ A\in M_{n\times n}(F):A_{i j}=0, i\leq j, A_{i j} = A_{j i} \right\} \\
			&= \left\{ \mathbf{O}_{n\times n} \right\}
		\end{align*}
		
		By definition of direct sum, we conclude $M_{n\times n}(F) = W_1\oplus W_2$.
	\end{proof}
\end{Exercise}