% === Exercise 1.6.29 ===
\begin{Exercise}
\begin{enumerate}[(a)]
\item
\begin{proof}
Follow the hint. First, we claim $\beta = \{u_1,\cdots,u_k,v_1,\cdots,v_m,w_1,\cdots,w_p\}$ is a basis for $W_1+W_2$. 
\begin{itemize}
\item $\mathbf{\boldsymbol{\beta}\ generates\ W_1+W_2}$.
\end{itemize}
Let 
\begin{align*}
t_1 &:= \sum_{i=1}^{k}a_i u_i + \sum_{i=1}^{m}b_i v_i\in W_1; \\
t_2 &:= \sum_{i=1}^{k}a'_i u_i + \sum_{i=1}^{p}c_i w_i\in W_2.
\end{align*}
Then pick $t = t_1+t_2 \in W_1+W_2$, we have 
$$
t = t_1+t_2 = \sum_{i=1}^{k}(a_i+a'_i) u_i + \sum_{i=1}^{m}b_i v_i + \sum_{i=1}^{p}c_i w_i \in span(\beta).
$$
Since $t_1$ and $t_2$ are arbitrary, this implies $W_1+W_2 =  span(\beta)$.

\begin{itemize}
\item $\mathbf{\boldsymbol{\beta}\ is\ linearly\ independent}$.
\end{itemize}
Consider
\begin{equation}\label{eq:ex_1.6.29a1}
\sum_{i=1}^{k}a_i u_i + \sum_{i=1}^{m}b_i v_i + \sum_{i=1}^{p}c_i w_i = 0.
\end{equation}
Let
\begin{equation}\label{eq:ex_1.6.29a2}
v := \sum_{i=1}^{k}a_i u_i \sum_{i=1}^{m}b_i v_i = -\sum_{i=1}^{p}c_i w_i.
\end{equation}
We know $v\in W_1$ and $v\in W_2$; hence $v\in W_1\cap W_2$. It follows that
$$
v = \sum_{i=1}^{k}a'_i u_i.
$$
Since $\{u_1, \cdots, u_k, w_1, \cdots, w_p\}$ is a basis for $W_2$ and $v\in W_2$, then
$$
\sum_{i=1}^{k}a'_i u_i + \sum_{i=1}^{p}c_i w_i = 0
\implies
a'_1 = \cdots = a'_k = c_1 = \cdots = c_p = 0.
$$
Also since $\{u_1, \cdots, u_k, v_1, \cdots, v_m\}$ is a basis for $W_1$ and $v\in W_1$, from equation \eqref{eq:ex_1.6.29a2}, we know
$$
v = \sum_{i=1}^{k}a_i u_i \sum_{i=1}^{m}b_i v_i = 0
\implies
a_1 = \cdots = a_k = b_1 = \cdots = b_m = 0.
$$
Hence from equation \eqref{eq:ex_1.6.29a1}, we obtain $\beta$ is linearly independent.

We prove the claim holds as promised. Finally, we compute
\begin{align}
dim(W_1+W_2) 
&= k+m+p \notag \\
&= (k+m) + (k+p) - k \notag \\
&= dim(W_1) + dim(W_2) - dim(W_1\cap W_2). \label{eq:ex_1.6.29a3}
\end{align}

By hypothesis that $W_1,W_2$ are finite-dimensional vector spaces, we know $W_1\cap W_2$ is also finite-dimensional; hence we obtain $k+m,k+p,k<\infty$. From formula \eqref{eq:ex_1.6.29a3}, we conclude $W_1+W_2$ is also a finite-dimensional vector space since $k+m+p<\infty$.
\end{proof}

\item
\begin{proof}
From part (a) and by hypothesis, we know
$$
dim(W_1+W_2) = dim(W_1)+dim(W_2)-dim(W_1\cap W_2).
$$
Hence
\begin{alignat*}{7}
\quad&& V &= W_1\oplus W_2 \\
\iff&& V &= W_1+W_2\text{ and }W_1\cap W_2=\{0\} \\
\iff&& dim(V) &= dim(W_1)+dim(W_2)-dim(\{0\}) \\
\iff&& dim(V) &= dim(W_1)+dim(W_2)
\end{alignat*}
\end{proof}
\end{enumerate}
\end{Exercise}