% === Exercise 1.6.9 ===
\begin{Exercise}
\begin{answer}
$(a_1,a_2,a_3,a_4)=a_1 u_1 + (a_2-a_1) u_2 + (a_3-a_2) u_3 + (a_4-a_3) u_4$.
\end{answer}
\begin{solution}
Let $(a_1,a_2,a_3,a_4) := c_1 u_1 + c_2 u_2 + c_3 u_3 + c_4 u_4$ where $c_1, c_2, c_3, c_4\in F$. By hypothesis, we can compute to obtain
$$
c_1 u_1 + c_2 u_2 + c_3 u_3 + c_4 u_4 = (c_1, c_1+c_2, c_1+c_2+c_3,c_1+c_2+c_3+c_4).
$$
Then
$$
\begin{cases}
\begin{aligned}
a_1 &= c_1 \\
a_2 &= c_1+c_2 \\
a_3 &= c_1+c_2+c_3 \\
a_4 &= c_1+c_2+c_3+c_4
\end{aligned}
\end{cases}.
$$
Solve it to know $c_1 = a_1, c_2 = a_2-a_1, c_3 = a_3-a_2, c_4 = a_4-a_3$. Hence we conclude 
$$
(a_1,a_2,a_3,a_4)=a_1 u_1 + (a_2-a_1) u_2 + (a_3-a_2) u_3 + (a_4-a_3) u_4.
$$
\end{solution}
\end{Exercise}